computation/computation10.v
@@ -1,0 +1,140 @@
+(*
+
+  Copyright 2014 Cornell University
+  Copyright 2015 Cornell University
+  Copyright 2016 Cornell University
+
+  This file is part of VPrl (the Verified Nuprl project).
+
+  VPrl is free software: you can redistribute it and/or modify
+  it under the terms of the GNU General Public License as published by
+  the Free Software Foundation, either version 3 of the License, or
+  (at your option) any later version.
+
+  VPrl is distributed in the hope that it will be useful,
+  but WITHOUT ANY WARRANTY; without even the implied warranty of
+  MERCHANTABILITY or FITNESS FOR A PARTICULAR PURPOSE.  See the
+  GNU General Public License for more details.
+
+  You should have received a copy of the GNU General Public License
+  along with VPrl.  If not, see <http://www.gnu.org/licenses/>.
+
+
+  Websites: http://nuprl.org/html/verification/
+            http://nuprl.org/html/Nuprl2Coq
+            https://github.com/vrahli/NuprlInCoq
+
+  Authors: Vincent Rahli
+
+*)
+
+Require Export computation2.
+
+
+(* !! MOVE to opid *)
+Lemma dec_can_eq_lambda {o} :
+  forall (c : @CanonicalOp o),
+    decidable (c = NLambda).
+Proof.
+  introv; unfold decidable.
+  destruct c; tcsp; try (complete (right; sp; ginv)).
+Qed.
+
+(* !! MOVE to opid *)
+Lemma dec_can_eq_int {o} :
+  forall (can : @CanonicalOp o),
+    decidable ({i : Z & can = Nint i}).
+Proof.
+  introv.
+  destruct can; tcsp; try (complete (right; sp; ginv)).
+  left; eexists; eauto.
+Qed.
+
+(* !! MOVE to opid *)
+Lemma dec_op_eq_int {o} :
+  forall (op : @Opid o),
+    decidable ({i : Z & op = Can (Nint i)}).
+Proof.
+  introv.
+  destruct op; try (complete (right; sp; ginv)).
+  destruct c; tcsp; try (complete (right; sp; ginv)).
+  left; eexists; eauto.
+Qed.
+
+Lemma wf_term_ncompop_iff {p} :
+  forall o (bterms : list (@BTerm p)),
+    wf_term (oterm (NCan (NCompOp o)) bterms)
+    <=> {a : NTerm
+        $ {b : NTerm
+        $ {c : NTerm
+        $ {d : NTerm
+           $ bterms = [bterm [] a, bterm [] b, bterm [] c, bterm [] d]
+           # wf_term a
+           # wf_term b
+           # wf_term c
+           # wf_term d}}}}.
+Proof.
+  introv.
+  rw @wf_oterm_iff; simpl; split; intro k; exrepnd.
+  - repeat (destruct bterms; allsimpl; ginv).
+    allunfold @num_bvars.
+    destruct b, b0, b1, b2; allsimpl.
+    destruct l; allsimpl; ginv.
+    destruct l0; allsimpl; ginv.
+    destruct l1; allsimpl; ginv.
+    destruct l2; allsimpl; ginv.
+    pose proof (k (bterm [] n))  as h1; autodimp h1 hyp.
+    pose proof (k (bterm [] n0)) as h2; autodimp h2 hyp.
+    pose proof (k (bterm [] n1)) as h3; autodimp h3 hyp.
+    pose proof (k (bterm [] n2)) as h4; autodimp h4 hyp.
+    allrw @wf_bterm_iff.
+    exists n n0 n1 n2; sp.
+  - repeat (destruct bterms; allsimpl; ginv).
+    unfold num_bvars; simpl; dands; auto.
+    introv i; repndors; tcsp; subst; allrw @wf_bterm_iff; auto.
+Qed.
+
+Lemma wf_term_narithop_iff {p} :
+  forall o (bterms : list (@BTerm p)),
+    wf_term (oterm (NCan (NArithOp o)) bterms)
+    <=> {a : NTerm
+        $ {b : NTerm
+           $ bterms = [bterm [] a, bterm [] b]
+           # wf_term a
+           # wf_term b}}.
+Proof.
+  introv.
+  rw @wf_oterm_iff; simpl; split; intro k; exrepnd.
+  - repeat (destruct bterms; allsimpl; ginv).
+    allunfold @num_bvars.
+    destruct b, b0; allsimpl.
+    destruct l; allsimpl; ginv.
+    destruct l0; allsimpl; ginv.
+    pose proof (k (bterm [] n))  as h1; autodimp h1 hyp.
+    pose proof (k (bterm [] n0)) as h2; autodimp h2 hyp.
+    allrw @wf_bterm_iff.
+    exists n n0; sp.
+  - repeat (destruct bterms; allsimpl; ginv).
+    unfold num_bvars; simpl; dands; auto.
+    introv i; repndors; tcsp; subst; allrw @wf_bterm_iff; auto.
+Qed.
+
+Lemma wf_minus {o} :
+  forall (t : @NTerm o),
+    wf_term (mk_minus t) <=> wf_term t.
+Proof.
+  introv.
+  unfold mk_minus.
+  rw @wf_oterm_iff; simpl; unfold num_bvars; simpl.
+  split; intro k; repnd; dands; tcsp; GC.
+  - pose proof (k (nobnd t)) as h; autodimp h hyp.
+  - introv i; repndors; tcsp; subst.
+    rw @wf_bterm_iff; auto.
+Qed.
+
+
+(*
+*** Local Variables:
+*** coq-load-path: ("." "../util/" "../terms/")
+*** End:
+*)
