continuity/continuity_defs.v
@@ -34,38 +34,9 @@ Require Export list_tacs.
 Require Export alphaeq2.
 Require Export substitution2.
 Require Export terms4.
+Require Export computation10.
 Require Export nat_defs.
 
-
-(* !! MOVE to opid *)
-Lemma dec_can_eq_lambda {o} :
-  forall (c : @CanonicalOp o),
-    decidable (c = NLambda).
-Proof.
-  introv; unfold decidable.
-  destruct c; tcsp; try (complete (right; sp; ginv)).
-Qed.
-
-(* !! MOVE to opid *)
-Lemma dec_can_eq_int {o} :
-  forall (can : @CanonicalOp o),
-    decidable ({i : Z & can = Nint i}).
-Proof.
-  introv.
-  destruct can; tcsp; try (complete (right; sp; ginv)).
-  left; eexists; eauto.
-Qed.
-
-(* !! MOVE to opid *)
-Lemma dec_op_eq_int {o} :
-  forall (op : @Opid o),
-    decidable ({i : Z & op = Can (Nint i)}).
-Proof.
-  introv.
-  destruct op; try (complete (right; sp; ginv)).
-  destruct c; tcsp; try (complete (right; sp; ginv)).
-  left; eexists; eauto.
-Qed.
 
 
 
@@ -2772,77 +2743,6 @@ Lemma free_vars_subst_utokens_aux_subset {o} :
 Proof.
   introv.
   rw <- subvars_eq; apply free_vars_subst_utokens_aux.
-Qed.
-
-Lemma wf_term_ncompop_iff {p} :
-  forall o (bterms : list (@BTerm p)),
-    wf_term (oterm (NCan (NCompOp o)) bterms)
-    <=> {a : NTerm
-        $ {b : NTerm
-        $ {c : NTerm
-        $ {d : NTerm
-           $ bterms = [bterm [] a, bterm [] b, bterm [] c, bterm [] d]
-           # wf_term a
-           # wf_term b
-           # wf_term c
-           # wf_term d}}}}.
-Proof.
-  introv.
-  rw @wf_oterm_iff; simpl; split; intro k; exrepnd.
-  - repeat (destruct bterms; allsimpl; ginv).
-    allunfold @num_bvars.
-    destruct b, b0, b1, b2; allsimpl.
-    destruct l; allsimpl; ginv.
-    destruct l0; allsimpl; ginv.
-    destruct l1; allsimpl; ginv.
-    destruct l2; allsimpl; ginv.
-    pose proof (k (bterm [] n))  as h1; autodimp h1 hyp.
-    pose proof (k (bterm [] n0)) as h2; autodimp h2 hyp.
-    pose proof (k (bterm [] n1)) as h3; autodimp h3 hyp.
-    pose proof (k (bterm [] n2)) as h4; autodimp h4 hyp.
-    allrw @wf_bterm_iff.
-    exists n n0 n1 n2; sp.
-  - repeat (destruct bterms; allsimpl; ginv).
-    unfold num_bvars; simpl; dands; auto.
-    introv i; repndors; tcsp; subst; allrw @wf_bterm_iff; auto.
-Qed.
-
-Lemma wf_term_narithop_iff {p} :
-  forall o (bterms : list (@BTerm p)),
-    wf_term (oterm (NCan (NArithOp o)) bterms)
-    <=> {a : NTerm
-        $ {b : NTerm
-           $ bterms = [bterm [] a, bterm [] b]
-           # wf_term a
-           # wf_term b}}.
-Proof.
-  introv.
-  rw @wf_oterm_iff; simpl; split; intro k; exrepnd.
-  - repeat (destruct bterms; allsimpl; ginv).
-    allunfold @num_bvars.
-    destruct b, b0; allsimpl.
-    destruct l; allsimpl; ginv.
-    destruct l0; allsimpl; ginv.
-    pose proof (k (bterm [] n))  as h1; autodimp h1 hyp.
-    pose proof (k (bterm [] n0)) as h2; autodimp h2 hyp.
-    allrw @wf_bterm_iff.
-    exists n n0; sp.
-  - repeat (destruct bterms; allsimpl; ginv).
-    unfold num_bvars; simpl; dands; auto.
-    introv i; repndors; tcsp; subst; allrw @wf_bterm_iff; auto.
-Qed.
-
-Lemma wf_minus {o} :
-  forall (t : @NTerm o),
-    wf_term (mk_minus t) <=> wf_term t.
-Proof.
-  introv.
-  unfold mk_minus.
-  rw @wf_oterm_iff; simpl; unfold num_bvars; simpl.
-  split; intro k; repnd; dands; tcsp; GC.
-  - pose proof (k (nobnd t)) as h; autodimp h hyp.
-  - introv i; repndors; tcsp; subst.
-    rw @wf_bterm_iff; auto.
 Qed.
 
 Lemma wf_force_int_bound {o} :
